prove hoare_abstract_method_intro'

core/ConcreteHoare.v
@@ -574,7 +574,7 @@ Proof.
     }
     eapply Forall2_sym; [ | eassumption].
     eapply exec_val_sym.
-    sauto.
+    clear; sauto.
   - eauto.
   - eauto.
 Qed.
@@ -657,6 +657,45 @@ Proof.
   unfold ARG.
   intros * [].
   eassumption.
+Qed.
+
+Definition AM_ARG (a_arg : list Sval) (a : extern_state -> Prop) :=
+  fun args es => arg_denote a_arg args /\ a es.
+
+Definition AM_ARG_RET (a_arg : list Sval) (a_ret : Sval) (a : extern_state -> Prop) :=
+  fun args retv es => arg_denote a_arg args
+    /\ ret_denote a_ret retv
+    /\ a es.
+
+Lemma hoare_abstract_method_intro' : forall am_ge p fd pre_arg pre_ext (func : AbsMet) post_arg
+    post_retv post_mem post_ext,
+  hoare_func am_ge p
+    (ARG pre_arg (MEM [] (EXT pre_ext)))
+    fd []
+    (ARG_RET post_arg post_retv (MEM post_mem (EXT post_ext))) ->
+  hoare_abstract_method
+    (AM_ARG pre_arg (ext_denote pre_ext))
+    (exec_abstract_method am_ge p fd)
+    (AM_ARG_RET post_arg post_retv (ext_denote post_ext)).
+Proof.
+  unfold hoare_func, hoare_abstract_method; intros.
+  inv H3.
+  eapply H0 in H6.
+  2 : {
+    split.
+    destruct H1.
+    2 : { simpl. sfirstorder. }
+    eapply Forall2_trans; [ | eassumption | eapply Forall2_trans; [ | eassumption | eassumption ]].
+    { refine sval_refine_trans. }
+    { refine sval_to_val_to_sval. }
+  }
+  destruct sig; inv H6.
+  unfold AM_ARG_RET.
+  intuition.
+  2 : { destruct H9; auto. }
+  eapply Forall2_trans; [ | eassumption | eapply Forall2_trans; [ | eassumption | eassumption ]].
+  { refine sval_refine_trans. }
+  { refine sval_to_val_to_sval. }
 Qed.
 
 End ConcreteHoare.
